Objectified blood records

bloodRep.dfy
@@ -2,7 +2,14 @@ include "dateRep.dfy"
 module BloodRep {
   import D = DateRep
   datatype BloodType = A | B | AB | O // A = 0, B = 1, AB = 2, O = 3
-  datatype BloodRecord = BloodRecord(bType: BloodType, location: string, donationDate: D.Date, expiryDate: D.Date, isOkay: bool)
+  
+  method createBt(bType: int) returns(bt: BloodType)
+  {
+    if(bType == 0) {return A;}
+    if(bType == 1) {return B;}
+    if(bType == 2) {return AB;}
+    if(bType == 3) {return O;}
+  }
 
   predicate typeValid(req: BloodType, ret: BloodType)
   {
@@ -12,15 +19,149 @@ module BloodRep {
     case O => (ret == O)
     case AB => (ret == AB || ret == A || ret == B || ret == O)
   }
-  
-  method createBt(bType: int) returns(bt: BloodType)
+
+  method getBTasString(bt: BloodType) returns(s: string)
   {
-    if(bType == 0) {return A;}
-    if(bType == 1) {return B;}
-    if(bType == 2) {return AB;}
-    if(bType == 3) {return O;}
+    match bt
+    case A => return "A";
+    case B => return "B";
+    case AB => return "AB";
+    case O => return "O";
   }
+
+  method getBTasInt(bt: BloodType) returns(i: int)
+  {
+    match bt
+    case A => return 1;
+    case B => return 2;
+    case AB => return 3;
+    case O => return 4;
+  }
+
+  class BloodRecord
+  {
+    var bType: BloodType, location: string, donationDate: D.Date, expiryDate: D.Date, isOkay: bool;
+    
+    predicate Valid()
+    reads this;
+    { 
+      D.validDate(donationDate.day, donationDate.month, donationDate.year) && D.validDate(expiryDate.day, expiryDate.month, expiryDate.year)
+    }
+
+    constructor(bt: BloodType, l: string, dd1: int,mm1:int,yy1:int, dd2:int,mm2:int,yy2:int, ok: bool)
+    modifies this;
+    requires D.validDate(dd1, mm1, yy1)
+    requires D.validDate(dd2, mm2, yy2)
+    ensures Valid();
+    ensures bType == bt;
+    ensures location == l;
+    ensures donationDate.day == dd1;
+    ensures donationDate.month== mm1;
+    ensures donationDate.year == yy1;
+    ensures expiryDate.day == dd2;
+    ensures expiryDate.month== mm2;
+    ensures expiryDate.year == yy2;
+    ensures isOkay == ok;
+    { 
+      bType := bt; 
+      location := l; 
+      donationDate := D.create(dd1,mm1,yy1); 
+      expiryDate := D.create(dd2,mm2,yy2); 
+      isOkay := ok;
+    }
+
+    // Current date is set as 22 Nov 2019
+    method hasExpired() returns (b: bool)
+    ensures !b <==> (2019 < expiryDate.year) 
+              || (2019 == expiryDate.year && 11 < expiryDate.month) 
+              || (2019 == expiryDate.year && 11 == expiryDate.month && 22 < expiryDate.day) 
+    {
+      var d1 := expiryDate;
+      var current := D.create(22, 11, 2019);
+      // Tests whether it has not expired
+      b := D.lessThan(current, expiryDate);
+      // Get opposite 
+      b := !b;
+    }
+
+    predicate placeholderPredicate()
+    reads this
+    {
+      (2019 < expiryDate.year) 
+          || (2019 == expiryDate.year && 11 < expiryDate.month) 
+          || (2019 == expiryDate.year && 11 == expiryDate.month && 22 < expiryDate.day) 
+    }
+ 
+    method notValid()
+    modifies this
+    ensures !placeholderPredicate() ==> !isOkay
+    {
+      var expire := hasExpired();
+      if (expire) { 
+        isOkay := false;
+      }
+    }
+
+    method compare(b2: BloodRecord) returns (cmp: int)
+    requires b2 != null
+    ensures (cmp == -1) <==> (expiryDate.year < b2.expiryDate.year) 
+                          || (expiryDate.year == b2.expiryDate.year && expiryDate.month < b2.expiryDate.month) 
+                          || (expiryDate.year == b2.expiryDate.year && expiryDate.month == b2.expiryDate.month && expiryDate.day < b2.expiryDate.day)  
+    ensures (cmp == 0) <==> (expiryDate.year == b2.expiryDate.year && expiryDate.month == b2.expiryDate.month && expiryDate.day == b2.expiryDate.day)
+
+    ensures (cmp == 1) <==> (b2.expiryDate.year < expiryDate.year) 
+                         || (b2.expiryDate.year == expiryDate.year && b2.expiryDate.month < expiryDate.month) 
+                         || (b2.expiryDate.year == expiryDate.year && b2.expiryDate.month == expiryDate.month && b2.expiryDate.day < expiryDate.day)
+    {
+      var a := D.lessThan(expiryDate, b2.expiryDate);
+      var b := D.lessThan(b2.expiryDate, expiryDate);
+      assert( a ==> !b && b ==> !a);
+      if (a) { return -1; } 
+      else if (b) { return 1; }
+      else { return 0; }
+    }
+  }
+
   
+
+
+  
+  method Test() 
+  {
+    var typeA := createBt(0);
+    var typeB := createBt(1);
+    var typeAB := createBt(2);
+    var typeO := createBt(3);
+    
+    //var br1 := createBr(typeA, "Backyard", 4, 2, 2003, 12, 4, 2007, true);
+    //var br2 := createBr(typeA, "Backyard", 1, 2, 2013, 11, 5, 2015, true);
+    var br1 := new BloodRecord(typeA, "Backyard", 4, 2, 2003, 12, 4, 2007, true);
+    var br2 := new BloodRecord(typeA, "Backyard", 1, 2, 2013, 11, 5, 2015, true);
+
+    var test1 := br1.hasExpired();
+    var test2 := br1.compare(br1);
+    var test3 := br1.compare(br2);
+    var test4 := br2.compare(br1);
+
+    assert(test1);    
+    assert(test2 == 0); 
+    assert(test4 == 1);
+    assert(test3 == -1);
+  }
+    
+
+}
+
+
+
+// HERE BE DRAGONS
+// AND OTHER RELICS OF THE PAST
+
+
+  //datatype BloodRecord = BloodRecord(bType: BloodType, location: string, donationDate: D.Date, expiryDate: D.Date, isOkay: bool)
+
+
+  /*
   // Create a blood record
   // TODO make a date addition to automatically set expiry date rather than pass through
   method createBr(bt: BloodType, l: string, dd1:int,mm1:int,yy1:int, dd2:int,mm2:int,yy2:int, isOkay: bool) returns (br: BloodRecord)
@@ -41,75 +182,27 @@ module BloodRep {
     br := BloodRecord(bt, l, d1, d2, isOkay);
   }
  
-  // Current date is set as 22 Nov 2019
-  method hasExpired(b1: BloodRecord) returns (b: bool)
-  ensures !b <==> (2019 < b1.expiryDate.year) 
-              || (2019 == b1.expiryDate.year && 11 < b1.expiryDate.month) 
-              || (2019 == b1.expiryDate.year && 11 == b1.expiryDate.month && 22 < b1.expiryDate.day) 
-  {
-    var d1 := b1.expiryDate;
-    var current := D.create(22, 11, 2019);
-    // Tests whether it has not expired
-    b := D.lessThan(current, b1.expiryDate);
-    // Get opposite 
-    b := !b;
-  }
+  */
 
-  method compare(b1: BloodRecord, b2: BloodRecord) returns (cmp: int)
-  ensures (cmp == -1) <==> (b1.expiryDate.year < b2.expiryDate.year) 
-                       || (b1.expiryDate.year == b2.expiryDate.year && b1.expiryDate.month < b2.expiryDate.month) 
-                       || (b1.expiryDate.year == b2.expiryDate.year && b1.expiryDate.month == b2.expiryDate.month && b1.expiryDate.day < b2.expiryDate.day)  
-  ensures (cmp == 0) <==> (b1.expiryDate.year == b2.expiryDate.year && b1.expiryDate.month == b2.expiryDate.month && b1.expiryDate.day == b2.expiryDate.day)
 
-  ensures (cmp == 1) <==> (b2.expiryDate.year < b1.expiryDate.year) 
-                       || (b2.expiryDate.year == b1.expiryDate.year && b2.expiryDate.month < b1.expiryDate.month) 
-                       || (b2.expiryDate.year == b1.expiryDate.year && b2.expiryDate.month == b1.expiryDate.month && b2.expiryDate.day < b1.expiryDate.day)
-  {
-    var a := D.lessThan(b1.expiryDate, b2.expiryDate);
-    var b := D.lessThan(b2.expiryDate, b1.expiryDate);
-    assert( a ==> !b && b ==> !a);
-    if (a) { return -1; } 
-    else if (b) { return 1; }
-    else { return 0; }
-  }
-  
-  method Test() 
-  {
-    var typeA := createBt(0);
-    var typeB := createBt(1);
-    var typeAB := createBt(2);
-    var typeO := createBt(3);
-    
-    var br1 := createBr(typeA, "Backyard", 4, 2, 2003, 12, 4, 2007, true);
-    var br2 := createBr(typeA, "Backyard", 1, 2, 2013, 11, 5, 2015, true);
+/*
+   (  )   /\   _                 (     
+    \ |  (  \ ( \.(               )                      _____
+  \  \ \  `  `   ) \             (  ___                 / _   \
+ (_`    \+   . x  ( .\            \/   \____-----------/ (o)   \_
+- .-               \+  ;          (  O                           \____
+                          )        \_____________  `              \  /
+(__                +- .( -'.- <. - _  VVVVVVV VV V\                 \/
+(_____            ._._: <_ - <- _  (--  _AAAAAAA__A_/                  |
+  .    /./.+-  . .- /  +--  - .     \______________//_              \_______
+  (__ ' /x  / x _/ (                                  \___'          \     /
+ , x / ( '  . / .  /                                      |           \   /
+    /  /  _/ /    +                                      /              \/
+   '  (__/                                             /                  \
 
-    var test1 := hasExpired(br1);
-    var test2 := compare(br1, br1);
-    var test3 := compare(br1, br2);
-    var test4 := compare(br2, br1);
+*/
 
-    assert(test1);    
-    assert(test2 == 0); 
-    assert(test4 == 1);
-    assert(test3 == -1);
-  }
-    
-  method getBTasString(bt: BloodType) returns(s: string)
-  {
-    match bt
-    case A => return "A";
-    case B => return "B";
-    case AB => return "AB";
-    case O => return "O";
-  }
 
-  method getBTasInt(bt: BloodType) returns(i: int)
-  {
-    match bt
-    case A => return 1;
-    case B => return 2;
-    case AB => return 3;
-    case O => return 4;
-  }
 
-}
+
+
